WIP algebra for an Oxide-like language

languages/with-user-builtins/myalgebra.v
@@ -3,15 +3,72 @@ From Minuska Require Import
   default_everything
 .
 
-Inductive Emptyset : Set := .
+(*  Oxide values *)
+Inductive Value :=
+| v_dead
+| v_z (z : Z)
+.
+
+Definition Identifier := string.
+Definition StackFrame := gmap Identifier Value.
+Definition Stack := list StackFrame.
+
+(* Minuska's values (forming a primitive-value-algebra) *)
+Inductive PrimitiveValue :=
+| pv_err
+| pv_bool (b : bool)
+| pv_z (z : Z)
+| pv_ident (x : Identifier)
+| pv_value (v : Value)
+| pv_stackframe (f : StackFrame)
+| pv_stack (s : Stack)
+.
+
+
+Variant PredicateSymbol :=
+| ps_is_value
+| ps_is_stack
+| ps_stack_is_empty
+| ps_stack_is_nonempty
+| ps_bool_is_true
+| ps_bool_is_false
+.
+
+Variant FunctionSymbol :=
+| fs_bool_neg (* bool -> bool *)
+| fs_stack_head (* Stack -> StackFrame *)
+| fs_stack_tail (* Stack -> Stack *)
+| fs_stack_push (* Stack -> StackFrame -> Stack *)
+| fs_frame_has (* StackFrame -> Identifier -> bool *)
+| fs_frame_lookup (* StackFrame -> Identifier -> Value *)
+| fs_frame_insert (* StackFrame -> Identifier -> Value -> StackFrame *)
+| fs_frame_delete (* StackFrame -> Identifier -> StackFrame *)
+.
+
 
 #[export]
-Instance emptyset_eqdec : EqDecision Emptyset.
+Instance Value_eqdec : EqDecision Value.
 Proof.
-    intros x y.
-    destruct x, y.
+  ltac1:(solve_decision).
 Defined.
 
+#[export]
+Instance PrimitiveValue_eqdec : EqDecision PrimitiveValue.
+Proof.
+  ltac1:(solve_decision).
+Defined.
+
+#[export]
+Instance PredicateSymbol_eqdec : EqDecision PredicateSymbol.
+Proof.
+  ltac1:(solve_decision).
+Defined.
+
+#[export]
+Instance FunctionSymbol_eqdec : EqDecision FunctionSymbol.
+Proof.
+  ltac1:(solve_decision).
+Defined.
 
 Section sec.
 
@@ -25,15 +82,27 @@ Section sec.
     Instance β
         : Builtin MyUnit := {|
         builtin_value
-            := Emptyset ;
+            := PrimitiveValue ;
         builtin_function_symbol
-            := Emptyset ;
+            := FunctionSymbol ;
         builtin_predicate_symbol
-            := Emptyset ;
+            := PredicateSymbol ;
         builtin_function_interp
-            := fun p => match p with end ;
+            := fun
+              (f : FunctionSymbol)
+              (nd : _)
+              (args : list (TermOver' PrimitiveValue))
+              => (t_over pv_err)
+        ;
+
         builtin_predicate_interp
-            := fun p => match p with end ;
+            := fun
+              (p : PredicateSymbol)
+              (nd : _)
+              (args : list (TermOver' PrimitiveValue))
+              =>
+              false
+        ;
     |}.
 
 End sec.
@@ -44,40 +113,47 @@ Definition builtins_binding : BuiltinsBinding := {|
 
 Definition inject_bool
     {symbol : Type}
-    (Fret : option Emptyset -> Emptyset)
+    (Fret : option PrimitiveValue -> PrimitiveValue)
     (b : bool)
     :
-    Emptyset :=
-    Fret None
+    PrimitiveValue :=
+    Fret (Some (pv_bool b))
 .
 
 Definition inject_Z
     {symbol : Type}
-    (Fret : option Emptyset -> Emptyset)
+    (Fret : option PrimitiveValue -> PrimitiveValue)
     (z : Z)
     :
-    Emptyset :=
-    Fret None
+    PrimitiveValue :=
+    Fret (Some (pv_z z))
 .
 
 Definition inject_string
     {symbol : Type}
-    (Fret : option Emptyset -> Emptyset)
+    (Fret : option PrimitiveValue -> PrimitiveValue)
     (s : string)
     :
-    Emptyset :=
-    Fret None
+    PrimitiveValue :=
+    Fret (Some (pv_ident s))
 .
 
 Definition eject
     {symbol : Type}
-    (v : Emptyset)
+    (v : PrimitiveValue)
     :
     option (bool+(Z+(string+unit)))%type
-    :=
-    None
+  :=
+    match v with
+    | pv_err => Some (inr (inr (inr tt)))
+    | pv_ident s => Some (inr (inr (inl s)))
+    | pv_bool b => Some (inl b)
+    | pv_value v' => None
+    | pv_z z => Some (inr (inl z))
+    | pv_stackframe _ => None
+    | pv_stack _ => None
+    end
 .
-
 
 Definition fancy_number := 5.
 
